Advancing lemmas on substitution/renamings

coq/theories/Examples/MuMuTilde.v
@@ -1,5 +1,5 @@
 From OGS Require Import Prelude.
-From OGS.Utils Require Import Ctx.
+From OGS.Utils Require Import Psh Rel Ctx.
 From OGS.Game Require Import Event.
 From OGS.ITree Require Import ITree Monad Delay.
 
@@ -62,90 +62,133 @@ with val0 : t_ctx -> ty0 -> Type :=
 with state : t_ctx -> Type :=
 | Cut {Γ a} : term Γ (t+ a) -> term Γ (t- a) -> state Γ
 .
+Scheme term_mut := Induction for term Sort Prop
+with val0_mut := Induction for val0 Sort Prop
+with state_mut := Induction for state Sort Prop.
+Check state_mut.
+Check val0_mut.
+
+Record syn_ind_args (P : forall (t : t_ctx) (t0 : ty), term t t0 -> Prop)
+                    (P0 : forall (t : t_ctx) (t0 : ty0), val0 t t0 -> Prop)
+                    (P1 : forall t : t_ctx, state t -> Prop) :=
+  {
+    ind_s_mu : forall (Γ : ctx ty) (a : ty0) (s : state (Γ ▶ t- a)), P1 (Γ ▶ t- a)%ctx s -> P Γ (t+ a) (Mu s) ;
+    ind_s_val : forall (Γ : t_ctx) (a : ty0) (v : val0 Γ a), P0 Γ a v -> P Γ (t+ a) (Val v) ;
+    ind_s_varn : forall (Γ : ctx ty) (a : ty0) (h : Γ ∋ t- a), P Γ (t- a) (VarN h) ;
+    ind_s_mu' : forall (Γ : ctx ty) (a : ty0) (s : state (Γ ▶ t+ a)), P1 (Γ ▶ t+ a)%ctx s -> P Γ (t- a) (Mu' s) ;
+    ind_s_zer : forall Γ : t_ctx, P Γ (t- Zer) ZerK ;
+    ind_s_app : forall (Γ : t_ctx) (a b : ty0) (v : val0 Γ a),
+        P0 Γ a v -> forall t : term Γ (t- b), P Γ (t- b) t -> P Γ (t- (a → b)) (App v t) ;
+    ind_s_fst : forall (Γ : t_ctx) (a b : ty0) (t : term Γ (t- a)),
+        P Γ (t- a) t -> P Γ (t- (a × b)) (Fst t) ;
+    ind_s_snd : forall (Γ : t_ctx) (a b : ty0) (t : term Γ (t- b)),
+        P Γ (t- b) t -> P Γ (t- (a × b)) (Snd t) ;
+    ind_s_match : forall (Γ : ctx ty) (a b : ty0) (s : state (Γ ▶ t+ a)),
+        P1 (Γ ▶ t+ a)%ctx s ->
+        forall s0 : state (Γ ▶ t+ b),
+        P1 (Γ ▶ t+ b)%ctx s0 -> P Γ (t- (a + b)) (Match s s0) ;
+    ind_s_varp : forall (Γ : ctx ty) (a : ty0) (h : Γ ∋ t+ a), P0 Γ a (VarP h) ;
+    ind_s_inl : forall (Γ : t_ctx) (a b : ty0) (v : val0 Γ a), P0 Γ a v -> P0 Γ (a + b) (Inl v) ;
+    ind_s_inr : forall (Γ : t_ctx) (a b : ty0) (v : val0 Γ b), P0 Γ b v -> P0 Γ (a + b) (Inr v) ;
+    ind_s_onei : forall Γ : t_ctx, P0 Γ One OneI ;
+    ind_s_lam : forall (Γ : ctx ty) (a b : ty0) (t : term (Γ ▶ t+ (a → b) ▶ t+ a) (t+ b)),
+        P (Γ ▶ t+ (a → b) ▶ t+ a)%ctx (t+ b) t -> P0 Γ (a → b) (LamRec t) ;
+    ind_s_pair : forall (Γ : t_ctx) (a b : ty0) (t : term Γ (t+ a)),
+        P Γ (t+ a) t ->
+        forall t0 : term Γ (t+ b), P Γ (t+ b) t0 -> P0 Γ (a × b) (Pair t t0) ;
+    ind_s_cut : forall (Γ : t_ctx) (a : ty0) (t : term Γ (t+ a)),
+      P Γ (t+ a) t -> forall t0 : term Γ (t- a), P Γ (t- a) t0 -> P1 Γ (Cut t t0)
+} .
+
+Lemma term_ind_mut P0 P1 P2 (arg : syn_ind_args P0 P1 P2)
+                   (t : t_ctx) (t0 : ty) (x : term t t0) : P0 t t0 x .
+  destruct arg; now apply (term_mut P0 P1 P2).
+Qed.
+
+Lemma val0_ind_mut P0 P1 P2 (arg : syn_ind_args P0 P1 P2)
+                   (t : t_ctx) (t0 : ty0) (x : val0 t t0) : P1 t t0 x .
+  destruct arg; now apply (val0_mut P0 P1 P2).
+Qed.
+
+Lemma state_ind_mut P0 P1 P2 (arg : syn_ind_args P0 P1 P2)
+                   (t : t_ctx) (x : state t) : P2 t x .
+  destruct arg; now apply (state_mut P0 P1 P2).
+Qed.
 
 Equations val : t_ctx -> ty -> Type :=
   val Γ (t+ a) := val0 Γ a ;
   val Γ (t- a) := term Γ (t- a) .
 
-Equations t_rename_aux {Γ Δ} ts : Γ ⊆ Δ -> term (Γ +▶ ts) ⇒ᵢ term (Δ +▶ ts) :=
-  t_rename_aux ts f _ (Mu c)    := Mu (s_rename_aux (ts ▶ _) f c) ;
-  t_rename_aux ts f _ (Val v)   := Val (v0_rename_aux ts f _ v) ;
-  t_rename_aux ts f _ (VarN i)  := VarN (r_shift_n ts f _ i) ;
-  t_rename_aux ts f _ (Mu' c)   := Mu' (s_rename_aux (ts ▶ _) f c) ;
-  t_rename_aux ts f _ (ZerK)    := ZerK ;
-  t_rename_aux ts f _ (App u k) := App (v0_rename_aux ts f _ u) (t_rename_aux ts f _ k) ;
-  t_rename_aux ts f _ (Fst k)   := Fst (t_rename_aux ts f _ k) ;
-  t_rename_aux ts f _ (Snd k)   := Snd (t_rename_aux ts f _ k) ;
-  t_rename_aux ts f _ (Match c1 c2) :=
-    Match (s_rename_aux (ts ▶ _) f c1)
-          (s_rename_aux (ts ▶ _) f c2)
-with v0_rename_aux {Γ Δ} ts : Γ ⊆ Δ -> val0 (Γ +▶ ts) ⇒ᵢ val0 (Δ +▶ ts) :=
-  v0_rename_aux ts f _ (VarP i)   := VarP (r_shift_n ts f _ i) ;
-  v0_rename_aux ts f _ (OneI)     := OneI ;
-  v0_rename_aux ts f _ (LamRec u) := LamRec (t_rename_aux (ts ▶ _ ▶ _) f _ u) ;
-  v0_rename_aux ts f _ (Pair u v) := Pair (t_rename_aux ts f _ u) (t_rename_aux ts f _ v) ;
-  v0_rename_aux ts f _ (Inl u)    := Inl (v0_rename_aux ts f _ u) ;
-  v0_rename_aux ts f _ (Inr u)    := Inr (v0_rename_aux ts f _ u)
-with s_rename_aux {Γ Δ} ts : Γ ⊆ Δ -> state (Γ +▶ ts) -> state (Δ +▶ ts) :=
-   s_rename_aux ts f (Cut v k) := Cut (t_rename_aux ts f _ v) (t_rename_aux ts f _ k) .
+Equations t_rename {Γ Δ} : Γ ⊆ Δ -> term Γ ⇒ᵢ term Δ :=
+  t_rename f _ (Mu c)    := Mu (s_rename (r_shift f) c) ;
+  t_rename f _ (Val v)   := Val (v0_rename f _ v) ;
+  t_rename f _ (VarN i)  := VarN (f _ i) ;
+  t_rename f _ (Mu' c)   := Mu' (s_rename (r_shift f) c) ;
+  t_rename f _ (ZerK)    := ZerK ;
+  t_rename f _ (App u k) := App (v0_rename f _ u) (t_rename f _ k) ;
+  t_rename f _ (Fst k)   := Fst (t_rename f _ k) ;
+  t_rename f _ (Snd k)   := Snd (t_rename f _ k) ;
+  t_rename f _ (Match c1 c2) :=
+    Match (s_rename (r_shift f) c1)
+          (s_rename (r_shift f) c2)
+with v0_rename {Γ Δ} : Γ ⊆ Δ -> val0 Γ ⇒ᵢ val0 Δ :=
+  v0_rename f _ (VarP i)   := VarP (f _ i) ;
+  v0_rename f _ (OneI)     := OneI ;
+  v0_rename f _ (LamRec u) := LamRec (t_rename (r_shift2 f) _ u) ;
+  v0_rename f _ (Pair u v) := Pair (t_rename f _ u) (t_rename f _ v) ;
+  v0_rename f _ (Inl u)    := Inl (v0_rename f _ u) ;
+  v0_rename f _ (Inr u)    := Inr (v0_rename f _ u)
+with s_rename {Γ Δ} : Γ ⊆ Δ -> state Γ -> state Δ :=
+   s_rename f (Cut v k) := Cut (t_rename f _ v) (t_rename f _ k) .
 
-Equations v_rename_aux {Γ Δ} ts : Γ ⊆ Δ -> val (Γ +▶ ts) ⇒ᵢ val (Δ +▶ ts) :=
-  v_rename_aux ts f (t+ _) v := v0_rename_aux ts f _ v ;
-  v_rename_aux ts f (t- _) k := t_rename_aux ts f _ k .
+Equations v_rename {Γ Δ} : Γ ⊆ Δ -> val Γ ⇒ᵢ val Δ :=
+  v_rename f (t+ _) v := v0_rename f _ v ;
+  v_rename f (t- _) k := t_rename f _ k .
 
 Equations Var {Γ} : has Γ ⇒ᵢ val Γ :=
   Var (t+ _) i := VarP i ;
   Var (t- _) i := VarN i .
-
-Definition t_rename  {Γ Δ} (f : Γ ⊆ Δ) := @t_rename_aux Γ Δ ∅ f.
-Definition v0_rename {Γ Δ} (f : Γ ⊆ Δ) := @v0_rename_aux Γ Δ ∅ f.
-Definition s_rename  {Γ Δ} (f : Γ ⊆ Δ) := @s_rename_aux Γ Δ ∅ f.
-Definition v_rename  {Γ Δ} (f : Γ ⊆ Δ) := @v_rename_aux Γ Δ ∅ f.
 
 Definition t_shift  {Γ} [y] : term Γ ⇒ᵢ term (Γ ▶ y)  := @t_rename _ _ s_pop.
 Definition v0_shift {Γ} [y] : val0 Γ ⇒ᵢ val0 (Γ ▶ y)  := @v0_rename _ _ s_pop.
 Definition s_shift  {Γ} [y] : state Γ -> state (Γ ▶ y) := @s_rename _ _ s_pop.
 Definition v_shift  {Γ} [y] : val Γ ⇒ᵢ val (Γ ▶ y)    := @v_rename _ _ s_pop.
 
+Definition a_shift {Γ Δ} [y] (a : Γ =[val]> Δ) : (Γ ▶ y) =[val]> (Δ ▶ y) :=
+  s_append (fun _ i => v_shift _ (a _ i)) (Var _ top).
+
+Definition a_shift2 {Γ Δ} [y z] (a : Γ =[val]> Δ) : (Γ ▶ y ▶ z) =[val]> (Δ ▶ y ▶ z) :=
+  a_shift (a_shift a).
+
 Equations t_of_v {Γ} : val Γ ⇒ᵢ term Γ :=
   t_of_v (t+ _) v := Val v ;
   t_of_v (t- _) k := k .
 
-Equations a_shift_n {Γ Δ} ts : Γ =[val]> Δ -> (Γ +▶ ts) =[val]> (Δ +▶ ts) :=
-  a_shift_n ts f _ i with cat_split i :=
-    { | CLeftV j := v_rename r_concat_l _ (f _ j) ;
-      | CRightV j := Var _ (r_concat_r _ j) } .
+Equations t_subst {Γ Δ} : Γ =[val]> Δ -> term Γ ⇒ᵢ term Δ :=
+  t_subst f _ (Mu c)    := Mu (s_subst (a_shift f) c) ;
+  t_subst f _ (Val v)   := Val (v0_subst f _ v) ;
+  t_subst f _ (VarN i)  := f _ i ;
+  t_subst f _ (Mu' c)   := Mu' (s_subst (a_shift f) c) ;
+  t_subst f _ (ZerK)    := ZerK ;
+  t_subst f _ (App u k) := App (v0_subst f _ u) (t_subst f _ k) ;
+  t_subst f _ (Fst k)   := Fst (t_subst f _ k) ;
+  t_subst f _ (Snd k)   := Snd (t_subst f _ k) ;
+  t_subst f _ (Match c1 c2) :=
+    Match (s_subst (a_shift f) c1)
+          (s_subst (a_shift f) c2)
+with v0_subst {Γ Δ} : Γ =[val]> Δ -> val0 Γ ⇒ᵢ val0 Δ :=
+  v0_subst f _ (VarP i)   := f _ i ;
+  v0_subst f _ (OneI)     := OneI ;
+  v0_subst f _ (LamRec u) := LamRec (t_subst (a_shift2 f) _ u) ;
+  v0_subst f _ (Pair u v) := Pair (t_subst f _ u) (t_subst f _ v) ;
+  v0_subst f _ (Inl u)    := Inl (v0_subst f _ u) ;
+  v0_subst f _ (Inr u)    := Inr (v0_subst f _ u)
+with s_subst {Γ Δ} : Γ =[val]> Δ -> state Γ -> state Δ :=
+   s_subst f (Cut v k) := Cut (t_subst f _ v) (t_subst f _ k) .
 
-Equations t_subst_aux {Γ Δ} ts : Γ =[val]> Δ -> term (Γ +▶ ts) ⇒ᵢ term (Δ +▶ ts) :=
-  t_subst_aux ts f _ (Mu c)    := Mu (s_subst_aux (ts ▶ _) f c) ;
-  t_subst_aux ts f _ (Val v)   := Val (v0_subst_aux ts f _ v) ;
-  t_subst_aux ts f _ (VarN i)  := a_shift_n ts f _ i ;
-  t_subst_aux ts f _ (Mu' c)   := Mu' (s_subst_aux (ts ▶ _) f c) ;
-  t_subst_aux ts f _ (ZerK)    := ZerK ;
-  t_subst_aux ts f _ (App u k) := App (v0_subst_aux ts f _ u) (t_subst_aux ts f _ k) ;
-  t_subst_aux ts f _ (Fst k)   := Fst (t_subst_aux ts f _ k) ;
-  t_subst_aux ts f _ (Snd k)   := Snd (t_subst_aux ts f _ k) ;
-  t_subst_aux ts f _ (Match c1 c2) :=
-    Match (s_subst_aux (ts ▶ _) f c1)
-          (s_subst_aux (ts ▶ _) f c2)
-with v0_subst_aux {Γ Δ} ts : Γ =[val]> Δ -> val0 (Γ +▶ ts) ⇒ᵢ val0 (Δ +▶ ts) :=
-  v0_subst_aux ts f _ (VarP i)   := a_shift_n ts f _ i ;
-  v0_subst_aux ts f _ (OneI)     := OneI ;
-  v0_subst_aux ts f _ (LamRec u) := LamRec (t_subst_aux (ts ▶ _ ▶ _) f _ u) ;
-  v0_subst_aux ts f _ (Pair u v) := Pair (t_subst_aux ts f _ u) (t_subst_aux ts f _ v) ;
-  v0_subst_aux ts f _ (Inl u)    := Inl (v0_subst_aux ts f _ u) ;
-  v0_subst_aux ts f _ (Inr u)    := Inr (v0_subst_aux ts f _ u)
-with s_subst_aux {Γ Δ} ts : Γ =[val]> Δ -> state (Γ +▶ ts) -> state (Δ +▶ ts) :=
-   s_subst_aux ts f (Cut v k) := Cut (t_subst_aux ts f _ v) (t_subst_aux ts f _ k) .
-
-Equations v_subst_aux {Γ Δ} ts : Γ =[val]> Δ -> val (Γ +▶ ts) ⇒ᵢ val (Δ +▶ ts) :=
-  v_subst_aux ts f (t+ _) v := v0_subst_aux ts f _ v ;
-  v_subst_aux ts f (t- _) k := t_subst_aux ts f _ k .
-
-Definition t_subst  {Γ Δ} (f : Γ =[val]> Δ) := @t_subst_aux Γ Δ ∅ f.
-Definition v0_subst {Γ Δ} (f : Γ =[val]> Δ) := @v0_subst_aux Γ Δ ∅ f.
-Definition s_subst  {Γ Δ} (f : Γ =[val]> Δ) := @s_subst_aux Γ Δ ∅ f.
-Definition v_subst  {Γ Δ} (f : Γ =[val]> Δ) := @v_subst_aux Γ Δ ∅ f.
+Equations v_subst {Γ Δ} : Γ =[val]> Δ -> val Γ ⇒ᵢ val Δ :=
+  v_subst f (t+ _) v := v0_subst f _ v ;
+  v_subst f (t- _) k := t_subst f _ k .
 
 Definition ass1 {Γ a} (v : val Γ a) : (Γ ▶ a) =[val]> Γ := s_append Var v .
 
@@ -171,9 +214,20 @@ Arguments FFst {Γ a b}.
 Arguments FSnd {Γ a b}.
 Arguments FMatch {Γ a b}.
 
+Equations f0_subst {Γ Δ} : Γ =[val]> Δ -> forcing0 Γ ⇒ᵢ forcing0 Δ :=
+  f0_subst f a (FZerK)        := FZerK ;
+  f0_subst f a (FApp v k)     := FApp (v0_subst f _ v) (t_subst f _ k) ;
+  f0_subst f a (FFst k)       := FFst (t_subst f _ k) ;
+  f0_subst f a (FSnd k)       := FSnd (t_subst f _ k) ;
+  f0_subst f a (FMatch s1 s2) := FMatch (s_subst (a_shift f) s1) (s_subst (a_shift f) s2) .
+
 Equations forcing : t_ctx -> ty -> Type :=
   forcing Γ (t+ a) := val0 Γ a ;
   forcing Γ (t- a) := forcing0 Γ a .
+
+Equations f_subst {Γ Δ} : Γ =[val]> Δ -> forcing Γ ⇒ᵢ forcing Δ :=
+  f_subst s (t+ a) v := v0_subst s a v ;
+  f_subst s (t- a) f := f0_subst s a f .
 
 Definition nf (Γ : t_ctx) : Type := { a : ty & (Γ ∋ a * forcing Γ (t_neg a))%type }.
 
@@ -335,7 +389,7 @@ Defined.
 
 Definition play {Γ : neg_ctx} (c : state Γ)
   : delay ({ m : pat' Γ & pat_dom' Γ m =[val]> Γ })
-  := bind_delay (eval c) (fun n => Ret' (p_of_nf n ,' p_dom_of_nf n)).
+  := fmap_delay (fun n => (p_of_nf n ,' p_dom_of_nf n)) (eval c).
 
 Definition emb {Γ} (m : pat' Γ) : state (Γ +▶ pat_dom' Γ m) .
   destruct m as [a [i v]]; cbn in *.
@@ -347,6 +401,225 @@ Definition emb {Γ} (m : pat' Γ) : state (Γ +▶ pat_dom' Γ m) .
     + refine (Val (v_rename r_concat_r _ (t_of_p v))).
     + refine (VarN (r_concat_l _ i)).
 Defined.
+
+Definition a_comp {Γ1 Γ2 Γ3} : Γ2 =[val]> Γ3 -> Γ1 =[val]> Γ2 -> Γ1 =[val]> Γ3 :=
+  fun f g _ i => v_subst f _ (g _ i) .
+
+(*
+Definition s_subst_aux_assoc {Γ1 Γ2 Γ3}
+  (f : Γ2 =[val]> Γ3) (g : Γ1 =[val]> Γ2)
+  ts (x : state (Γ1 +▶ ts))
+  : s_subst_aux ts f (s_subst_aux ts g x)
+  = s_subst_aux ts (a_comp f g) x .
+
+*)
+Search "rename".
+
+(*
+Definition t_rename_aux_assoc {Γ1 Γ2 Γ3} ts (f1 : Γ2 ⊆ Γ3) (f2 : Γ1 ⊆ Γ2)
+  a (t : term (Γ1 +▶ ts) a)
+  : t_rename_aux ts f1 a (t_rename_aux ts f2 a t)
+    = t_rename_aux ts (s_ren f1 f2) a t.
+dependent induction t.
+- cbn; f_equal.
+  induction t.
+*)
+About f_equal.
+
+Lemma f_equal2 [A B C : Type] (f : A -> B -> C) [x1 x2 : A] [y1 y2 : B]
+  : x1 = x2 -> y1 = y2 -> f x1 y1 = f x2 y2.
+  intros H1 H2.
+  rewrite H1, H2; reflexivity.
+Qed.
+
+Axiom HOLE : forall X : Prop, X .
+
+(* TODO: move to Utils/Ctx.v*)
+Lemma r_shift_n_assoc {Γ1 Γ2 Γ3 : t_ctx} ts (f1 : Γ2 ⊆ Γ3) (f2 : Γ1 ⊆ Γ2)
+  a (i : (Γ1 +▶ ts) ∋ a)
+  : r_shift_n ts f1 a (r_shift_n ts f2 a i)
+    = r_shift_n ts (s_ren f1 f2) a i.
+  induction ts.
+  - reflexivity.
+  - dependent elimination i.
+    + reflexivity.
+    + cbn; unfold s_pop, s_ren; f_equal; apply IHts.
+Qed.
+
+Definition t_ren_proper_P Γ a (t : term Γ a) : Prop :=
+  forall Δ (f1 f2 : Γ ⊆ Δ), f1 ≡ₐ f2 -> t_rename f1 a t = t_rename f2 a t .
+Definition v0_ren_proper_P Γ a (v : val0 Γ a) : Prop :=
+  forall Δ (f1 f2 : Γ ⊆ Δ), f1 ≡ₐ f2 -> v0_rename f1 a v = v0_rename f2 a v .
+Definition s_ren_proper_P Γ (s : state Γ) : Prop :=
+  forall Δ (f1 f2 : Γ ⊆ Δ), f1 ≡ₐ f2 -> s_rename f1 s = s_rename f2 s .
+Lemma ren_proper_prf : syn_ind_args t_ren_proper_P v0_ren_proper_P s_ren_proper_P.
+  econstructor.
+  all: unfold t_ren_proper_P, v0_ren_proper_P, s_ren_proper_P.
+  all: intros; cbn; auto; f_equal; auto; unfold r_shift2.
+  all: try apply H; try apply H0; try rewrite H0; try rewrite H1; try reflexivity.
+Qed.
+
+#[global] Instance t_ren_eq {Γ Δ}
+  : Proper (ass_eq _ _ ==> dpointwise_relation (fun a => eq ==> eq)) (@t_rename Γ Δ).
+intros f1 f2 H1 a x y ->; now apply (term_ind_mut _ _ _ ren_proper_prf).
+Qed.
+
+#[global] Instance v0_ren_eq {Γ Δ}
+  : Proper (ass_eq _ _ ==> dpointwise_relation (fun a => eq ==> eq)) (@v0_rename Γ Δ).
+intros f1 f2 H1 a x y ->; now apply (val0_ind_mut _ _ _ ren_proper_prf).
+Qed.
+
+#[global] Instance s_ren_eq {Γ Δ}
+  : Proper (ass_eq _ _ ==> eq ==> eq) (@s_rename Γ Δ).
+intros f1 f2 H1 x y ->; now apply (state_ind_mut _ _ _ ren_proper_prf).
+Qed.
+
+Definition t_ren_assoc_P Γ1 a (t : term Γ1 a) : Prop :=
+  forall Γ2 Γ3 (f1 : Γ2 ⊆ Γ3) (f2 : Γ1 ⊆ Γ2),
+    t_rename f1 a (t_rename f2 a t) = t_rename (s_ren f1 f2) a t.
+Definition v0_ren_assoc_P Γ1 a (v : val0 Γ1 a) : Prop :=
+  forall Γ2 Γ3 (f1 : Γ2 ⊆ Γ3) (f2 : Γ1 ⊆ Γ2),
+    v0_rename f1 a (v0_rename f2 a v) = v0_rename (s_ren f1 f2) a v.
+Definition s_ren_assoc_P Γ1 (s : state Γ1) : Prop :=
+  forall Γ2 Γ3 (f1 : Γ2 ⊆ Γ3) (f2 : Γ1 ⊆ Γ2),
+    s_rename f1 (s_rename f2 s) = s_rename (s_ren f1 f2) s.
+
+Lemma ren_assoc_prf : syn_ind_args t_ren_assoc_P v0_ren_assoc_P s_ren_assoc_P.
+  econstructor.
+  all: unfold t_ren_assoc_P, v0_ren_assoc_P, s_ren_assoc_P.
+  all: intros; cbn; (try reflexivity); f_equal; eauto; unfold r_shift2.
+  all: repeat rewrite r_shift_comp; eauto.
+  etransitivity.
+  apply H.
+  apply t_ren_eq; auto.
+  rewrite 2 r_shift_comp.
+  reflexivity.
+Qed.
+
+Lemma t_rename_assoc {Γ1 Γ2 Γ3} (f1 : Γ2 ⊆ Γ3) (f2 : Γ1 ⊆ Γ2) a (t : term Γ1 a)
+  : t_rename f1 a (t_rename f2 a t) = t_rename (s_ren f1 f2) a t.
+now apply (term_ind_mut _ _ _ ren_assoc_prf). Qed.
+Lemma v0_rename_assoc {Γ1 Γ2 Γ3} (f1 : Γ2 ⊆ Γ3) (f2 : Γ1 ⊆ Γ2) a (v : val0 Γ1 a)
+  : v0_rename f1 a (v0_rename f2 a v) = v0_rename (s_ren f1 f2) a v.
+now apply (val0_ind_mut _ _ _ ren_assoc_prf). Qed.
+Lemma s_rename_assoc {Γ1 Γ2 Γ3} (f1 : Γ2 ⊆ Γ3) (f2 : Γ1 ⊆ Γ2) (s : state Γ1)
+  : s_rename f1 (s_rename f2 s) = s_rename (s_ren f1 f2) s.
+now apply (state_ind_mut _ _ _ ren_assoc_prf). Qed.
+
+Definition t_ren_id_l_P Γ a (t : term Γ a) : Prop := t_rename r_id a t = t.
+Definition v0_ren_id_l_P Γ a (v : val0 Γ a) : Prop := v0_rename r_id a v = v.
+Definition s_ren_id_l_P Γ (s : state Γ) : Prop := s_rename r_id s = s.
+
+Lemma ren_id_l_prf : syn_ind_args t_ren_id_l_P v0_ren_id_l_P s_ren_id_l_P.
+  econstructor.
+  all: unfold t_ren_id_l_P, v0_ren_id_l_P, s_ren_id_l_P.
+  all: intros; cbn; (try reflexivity); f_equal; eauto; unfold r_shift2.
+  all: try rewrite r_shift_id; eauto.
+  rewrite <- H.
+  apply t_ren_eq; auto.
+  rewrite 2 r_shift_id; auto.
+Qed.
+
+Lemma t_ren_id_l {Γ} a (t : term Γ a) : t_rename r_id a t = t.
+now apply (term_ind_mut _ _ _ ren_id_l_prf). Qed.
+Lemma v0_ren_id_l {Γ} a (v : val0 Γ a) : v0_rename r_id a v = v.
+now apply (val0_ind_mut _ _ _ ren_id_l_prf). Qed.
+Lemma s_ren_id_l {Γ} (s : state Γ) : s_rename r_id s = s.
+now apply (state_ind_mut _ _ _ ren_id_l_prf). Qed.
+
+Lemma v_ren_id_r {Γ Δ} (f : Γ ⊆ Δ) a (i : Γ ∋ a) : v_rename f a (Var _ i) = Var _ (f _ i).
+destruct a; auto. Qed.
+  
+Definition t_sub_proper_P Γ a (t : term Γ a) : Prop :=
+  forall Δ (f1 f2 : Γ =[val]> Δ), f1 ≡ₐ f2 -> t_subst f1 a t = t_subst f2 a t .
+Definition v0_sub_proper_P Γ a (v : val0 Γ a) : Prop :=
+  forall Δ (f1 f2 : Γ =[val]> Δ), f1 ≡ₐ f2 -> v0_subst f1 a v = v0_subst f2 a v .
+Definition s_sub_proper_P Γ (s : state Γ) : Prop :=
+  forall Δ (f1 f2 : Γ =[val]> Δ), f1 ≡ₐ f2 -> s_subst f1 s = s_subst f2 s .
+Lemma sub_proper_prf : syn_ind_args t_sub_proper_P v0_sub_proper_P s_sub_proper_P.
+  econstructor.
+  all: unfold t_sub_proper_P, v0_sub_proper_P, s_sub_proper_P.
+  all: intros; cbn; auto; f_equal; auto; unfold a_shift2, a_shift.
+  all: try apply H; try apply H0; try rewrite H0; try rewrite H1; try reflexivity.
+  all: apply s_append_eq; auto.
+  all: intros ? i; try f_equal; try rewrite H0; try rewrite H1; auto.
+  apply s_append_eq; auto; intros ? i'; rewrite H0; auto.
+Qed.
+
+#[global] Instance t_sub_eq {Γ Δ}
+  : Proper (ass_eq _ _ ==> dpointwise_relation (fun a => eq ==> eq)) (@t_subst Γ Δ).
+intros f1 f2 H1 a x y ->; now apply (term_ind_mut _ _ _ sub_proper_prf).
+Qed.
+
+#[global] Instance v0_sub_eq {Γ Δ}
+  : Proper (ass_eq _ _ ==> dpointwise_relation (fun a => eq ==> eq)) (@v0_subst Γ Δ).
+intros f1 f2 H1 a x y ->; now apply (val0_ind_mut _ _ _ sub_proper_prf).
+Qed.
+
+#[global] Instance s_sub_eq {Γ Δ}
+  : Proper (ass_eq _ _ ==> eq ==> eq) (@s_subst Γ Δ).
+intros f1 f2 H1 x y ->; now apply (state_ind_mut _ _ _ sub_proper_prf).
+Qed.
+
+(*
+Definition t_sub_assoc_P Γ1 a (t : term Γ1 a) : Prop :=
+  forall Γ2 Γ3 (f1 : Γ2 =[val]> Γ3) (f2 : Γ1 =[val]> Γ2),
+    t_subst f1 a (t_subst f2 a t) = t_subst (a_comp f1 f2) a t.
+Definition v0_sub_assoc_P Γ1 a (v : val0 Γ1 a) : Prop :=
+  forall Γ2 Γ3 (f1 : Γ2 =[val]> Γ3) (f2 : Γ1 =[val]> Γ2),
+    v0_subst f1 a (v0_subst f2 a v) = v0_subst (a_comp f1 f2) a v.
+Definition s_sub_assoc_P Γ1 (s : state Γ1) : Prop :=
+  forall Γ2 Γ3 (f1 : Γ2 =[val]> Γ3) (f2 : Γ1 =[val]> Γ2),
+    s_subst f1 (s_subst f2 s) = s_subst (a_comp f1 f2) s.
+
+Lemma ren_assoc_prf : syn_ind_args t_ren_assoc_P v0_ren_assoc_P s_ren_assoc_P.
+  econstructor.
+  all: unfold t_ren_assoc_P, v0_ren_assoc_P, s_ren_assoc_P.
+  all: intros; cbn; (try reflexivity); f_equal; eauto; unfold r_shift2.
+  all: repeat rewrite r_shift_comp; eauto.
+  etransitivity.
+  apply H.
+  apply t_ren_eq; auto.
+  rewrite 2 r_shift_comp.
+  reflexivity.
+Qed.
+
+
+
+
+    v0_rename f1 a (v0_rename f2 a v) = v0_rename (s_ren f1 f2) a v.
+Definition s_ren_assoc_P Γ1 (s : state Γ1) : Prop :=
+  forall Γ2 Γ3 (f1 : Γ2 ⊆ Γ3) (f2 : Γ1 ⊆ Γ2),
+    s_rename f1 (s_rename f2 s) = s_rename (s_ren f1 f2) s.
+*)
+
+
+From Coinduction Require Import coinduction lattice rel tactics.
+From OGS.Utils Require Import Psh Rel.
+From OGS.ITree Require Import ITree Eq Monad.
+
+Definition play_split {Γ Δ : neg_ctx} (e : Γ =[val]> Δ)
+  (p : { m : pat' (Δ +▶ Γ) & pat_dom' (Δ +▶ Γ) m =[val]> (Δ +▶ Γ) })
+           : delay ({ m : pat' Δ & pat_dom' Δ m =[val]> Δ }).
+  destruct (cat_split (fst (projT2 (projT1 p)))).
+  - refine (Ret' ((_ ,' (i , snd (projT2 (projT1 p)))) ,' a_comp ([Var,e]) (projT2 p))).
+  - refine (Tau' _).
+    refine (play _).
+    refine (s_subst _ (emb (projT1 p))).
+    refine ([[Var,e], (a_comp ([Var,e]) (projT2 p))]).
+Defined.
+
+
+Definition clean_hyp {Γ Δ : neg_ctx} (c : state (Δ +▶ₛ Γ)) (e : Γ =[val]> Δ) :
+  play (s_subst ([Var,e]) c) ≊ bind_delay' (play c) (play_split e).
+  unfold play, bind_delay', iter_delay, fmap_delay, it_eq.
+  rewrite fmap_bind_com.
+  unfold bind.
+  revert Γ c e; coinduction R CIH; intros Γ c e.
+  dependent elimination c.
+  unfold s_subst.
+  remember ([Var,e]) as e'.
+  Admitted.
 
 From OGS.OGS Require Spec.
 
@@ -366,33 +639,49 @@ Defined.
 
 Definition ctx_to_s (Γ : ctx neg_ty) : neg_ctx := {| sub_elt := c_map sub_elt Γ ; sub_prf := ctx_allS Γ |}.
 
-Program Definition mu_machine : Spec.machine mu_spec :=
-  {| Spec.conf := fun Γ => state (ctx_to_s Γ) ;
-     Spec.val := fun Γ t => val (ctx_to_s Γ) t.(sub_elt) |} .
-Next Obligation.
-  refine (fmap_delay _ (@play (ctx_to_s Γ) X)).
-  intros [ [ a [ i m ] ] s ]; cbn in *.
-  destruct (view_has_map sub_elt Γ i); cbn in *.
-  unshelve refine ((x ,' (i , m)) ,' _). cbn.
-  intros ? j.
-  destruct (view_s_has_map _ _ j); cbn in *.
-  exact (s _ i0).
+Definition state' (Γ : ctx neg_ty) : Type := state (ctx_to_s Γ).
+Definition val' (Γ : ctx neg_ty) (a : neg_ty) : Type := val (ctx_to_s Γ) a.(sub_elt).
+
+Definition ugly_ass_1 {Γ} {x : neg_ty} (m : pat (t_neg (sub_elt x)))
+          (s : pat_dom m =[ val ]> ctx_to_s Γ)
+          : Spec.dom mu_spec m =[ val' ]> Γ .
+  intros ? j; destruct (view_s_has_map _ _ j); exact (s _ i).
 Defined.
-Next Obligation.
+
+Definition ugly_ass_2 {Γ Δ : ctx neg_ty} (s : Γ =[ val' ]> Δ)
+  : ctx_to_s Γ =[ val ]> ctx_to_s Δ.
+  intros ? j.
+  destruct (view_has_map _ _ j); exact (s _ i).
+Defined.
+
+Definition ugly_play {Γ}
+  (u : { m : pat' (ctx_to_s Γ) & pat_dom' _ m =[val]> ctx_to_s Γ })
+  : {m : Spec.msg' mu_spec Γ & Spec.dom' mu_spec m =[val']> Γ }.
+  destruct u as [ [ a [ i m ] ] s ].
+  destruct (view_has_map sub_elt Γ i).
+  unshelve refine ((x ,' (i , m)) ,' ugly_ass_1 m s).
+Defined.
+
+Definition ugly_emb Γ (m : Spec.msg' mu_spec Γ)
+  : state' (Γ +▶ Spec.dom' mu_spec m).
   destruct m as [ a [ i m ]].
+  unfold state'; cbn -[ctx_s_map].
   rewrite map_cat, <- ctx_s_to_ctx_eq.
   exact (emb (_ ,' (map_has _ _ i , m))).
 Defined.
-Next Obligation.
-  exact (Var _ (map_has _ _ X)).
-Defined.
-Next Obligation.
-  refine (v_subst _ _ X0).
-  intros ? j.
-  destruct (view_has_map _ _ j); exact (X _ i0).
-Defined.
-Next Obligation.
-  refine (s_subst _ X0).
-  intros ? j.
-  destruct (view_has_map _ _ j); exact (X _ i).
-Defined.
+
+Program Definition mu_machine : Spec.machine mu_spec :=
+  {| Spec.conf := state' ;
+     Spec.val := val' ;
+     Spec.eval := fun Γ c => fmap_delay ugly_play (@play (ctx_to_s Γ) c) ;
+     Spec.emb := ugly_emb ;
+     Spec.v_var := fun _ _ i => Var _ (map_has _ _ i) ;
+     Spec.v_sub := fun _ _ a _ v => v_subst (ugly_ass_2 a) _ v ;
+     Spec.c_sub := fun _ _ a s => s_subst (ugly_ass_2 a) s ;
+  |}.
+
+Lemma the_hyp {Γ Δ}
+  (c : @Spec.conf _ mu_machine (Δ +▶ Γ)%ctx)
+  (e : Γ =[@Spec.val _ mu_machine]> Δ)
+  : @Spec.eval_sub_1 _ mu_machine Γ Δ c e ≊ @Spec.eval_sub_2 _ mu_machine Γ Δ c e.
+Admitted.
