coq/theories/ITree/Delay.v
@@ -34,8 +34,47 @@ Definition bind_delay {I} {E : event I I} {X Y i}
   : delay X -> (X -> itree E Y i) -> itree E Y i
   := fun x f => bind (emb_delay x) (fun _ '(Fib x) => f x) .
 
+Definition bind_delay' {X Y}
+  : delay X -> (X -> delay Y) -> delay Y
+  := fun x f => bind x (fun 'T1_0 y => f y).
+
 Definition fmap_delay {X Y} (f : X -> Y) : delay X -> delay Y :=
   fmap (fun 'T1_0 => f) T1_0 .
 
 Definition iter_delay {X Y} : (X -> delay (X + Y)) -> X -> delay Y :=
   fun f => iter (fun 'T1_0 => f) T1_0 .
+
+(*
+From Coinduction Require Import coinduction lattice rel tactics.
+From OGS Require Import Utils.Rel.
+From OGS Require Import ITree.Eq.
+
+Lemma iter_unfold {X Y} (f : X -> delay (X + Y)) {x}
+  :
+      (iter_delay f x)
+  ≊
+      (bind_delay' (f x) (fun r => match r with
+                                 | inl x => tau_delay (iter_delay f x)
+                                 | inr y => ret_delay y end)).
+Proof.
+  apply (gfp_fp (it_eq_map ∅ₑ (eqᵢ _))).
+  cbn; destruct (_observe (f x)).
+  - change (iter _ T1_0 ?x) with (iter_delay f x).
+    destruct r; econstructor; auto.
+  - econstructor.
+    eapply (it_eq_up2bind_t (eqᵢ (fun _ => (X + Y)%type)) _).
+    econstructor.
+    reflexivity.
+    intros [] ? ? <-.
+    cbn.
+
+    cbv; reflexivity.
+    + econstructor; auto.
+    unfold
+  try econstructor; eauto.
+  unfold iter_delay at 1.
+  unfold bind_delay.
+  destruct (_observe (f x)).
+  destruct r
+
+*)
